elements_of_ll (Autograder)

state/Examples.fst
@@ -9,6 +9,8 @@ open Witnessable
 open FStar.Tactics
 open FStar.Ghost
 
+module FSet = FStar.FiniteSet.Base
+
 type grade =
 | NotGraded
 | MaxGrade
@@ -27,6 +29,8 @@ let grade_preorder : preorder grade = fun g1 g2 ->
   | _ -> g1 == g2
 
 (* TODO: two implementations of each : one with Type0 (pred) & one for HO contracts (ST effect) *)
+
+let max_length = pow2 32 - 1
 
 let no_cycles (ll: linkedList int) (h: heap) : Type0 = admit()
 let sorted (ll: linkedList int) (h: heap) : Type0 = admit()
@@ -49,35 +53,67 @@ let rec sorted_fuel (fuel:nat) (ll:linkedList int) (h:heap): Type0 =
       | LLNil -> True
       | LLCons y next -> x <= y /\ sorted_fuel (fuel - 1) tl h
 
-(* #push-options "--split_queries always"
+(*TODO: replace these with deep_predicate *)
+let rec deep_contains_ll (fuel: nat) (l: linkedList int) (h: heap): Type0 =
+  if fuel = 0 then False
+  else
+    match l with
+    | LLNil -> True
+    | LLCons x xsref -> 
+      h `contains` xsref /\ deep_contains_ll (fuel - 1) (sel h xsref) h
+
+(* Probably remove this *)
 let rec footprint_acc
   (#a: Type)
-  (l: linkedList a)
-  (h:heap)
+  (l: linkedList a) 
+  (h:heap) 
   (hdom:(FSet.set nat){forall (a:Type) (rel:_) (r:mref a rel). h `contains` r ==> addr_of r `FSet.mem` hdom})
-  (acc:(FSet.set nat){acc `FSet.subset` hdom}) :
+  (acc:(FSet.set nat){acc `FSet.subset` hdom}) : 
   GTot (FSet.set nat) (decreases (FSet.cardinality (hdom `FSet.difference` acc))) =
-  match l with
-  | Nil -> acc
-  | Cons x xsref ->
+  match l with 
+  | LLNil -> acc
+  | LLCons x xsref -> 
     if addr_of xsref `FSet.mem` acc then acc
     else begin
       assume (h `contains` xsref);
       let acc' = (acc `FSet.union` FSet.singleton (addr_of xsref)) in
       FSet.all_finite_set_facts_lemma ();
-      assert (acc' `FSet.subset` hdom);
+      (* assert (acc' `FSet.subset` hdom);
       assert ((hdom `FSet.difference` acc') `FSet.subset`
               (hdom `FSet.difference` acc));
       assert (~((hdom `FSet.difference` acc') `FSet.equal`
-              (hdom `FSet.difference` acc)));
-      assert (FSet.cardinality (hdom `FSet.difference` acc') <
-              FSet.cardinality (hdom `FSet.difference` acc));
-      footprint_acc (sel h xsref) h hdom acc'
+              (hdom `FSet.difference` acc))); 
+      assert (FSet.cardinality (hdom `FSet.difference` acc') < 
+              FSet.cardinality (hdom `FSet.difference` acc)); *)
+      footprint_acc (sel h xsref) h hdom acc' 
     end
-#pop-options *)
 
-let elements_of_ll (ll:linkedList int) (h:heap) : Set.set int = admit()
-(* elements_of_ll_acc ll h Set.empty *)
+(* let get_hdom h =
+  FSet.all_finite_set_facts_lemma ();
+  let rec aux (n:nat) : res:(FSet.set nat){forall i. 0 < i && i <= n ==> i `FSet.mem` res} =
+    if n = 0 then FSet.emptyset 
+    else FSet.singleton n `FSet.union` (aux (n-1)) in
+  aux ((fst h).next - 1) *)
+
+(* let footprint (#a: Type) (l: linkedList a) (h:heap) : GTot (Set.set nat) =
+  let hdom = get_hdom h in
+  FSet.all_finite_set_facts_lemma ();
+  assert (FSet.emptyset `FSet.subset` hdom);
+  let fp : FSet.set nat = footprint_acc l h hdom FSet.emptyset in
+  Set.as_set (FSet.set_as_list fp) *)
+
+let rec elements_of_ll_acc (fuel:nat) (ll:linkedList int) (h:heap) (acc: FSet.set int) : GTot (FSet.set int) =
+  if fuel = 0 then acc
+  else 
+    match ll with 
+    | LLNil -> acc
+    | LLCons v next -> 
+      let acc' = acc `union` singleton(v) in 
+      let tail = sel h next in 
+      elements_of_ll_acc (fuel - 1) tail h acc'
+
+let elements_of_ll (ll:linkedList int) (h:heap) (acc: FSet.set int) : GTot (FSet.set int) = 
+  elements_of_ll_acc max_length ll h FSet.emptyset
 
 let same_elements (ll:linkedList int) (h0 h1:heap) = elements_of_ll ll h0 == elements_of_ll ll h1
 
@@ -105,26 +141,30 @@ let rec generate_llist (l:list int)
     (ensures (fun h0 r h1 -> satisfy_on_heap r h1 contains_pred)) =
   match l with
   | [] -> LLNil
-  | hd::tl -> LLCons hd (sst_alloc #(SLList SNat) (generate_llist tl)) (* sst_alloc or sst_alloc'? *)
+  | hd::tl -> LLCons hd (sst_alloc_shareable #(SLList SNat) (generate_llist tl))
 
-let rec deep_contains_ll (fuel: nat) (l: linkedList int) (h: heap): Type0 =
+let rec deep_private_ll (fuel: nat) (l: linkedList int) (h: heap): Type0 =
   if fuel = 0 then False
   else
     match l with
     | LLNil -> True
     | LLCons x xsref -> 
-      h `contains` xsref /\ deep_contains_ll (fuel - 1) (sel h xsref) h  
+      is_private xsref h /\ deep_private_ll (fuel - 1) (sel h xsref) h   
 
 let rec share_llist (l:linkedList int) 
   : SST unit 
-    (requires (fun h0 -> (exists fuel . deep_contains_ll fuel l h0)))
+    (requires (fun h0 -> (exists fuel . deep_contains_ll fuel l h0) /\ 
+                         (exists fuel . deep_private_ll fuel l h0)))
     (fun h0 r h1 -> True) = 
   match l with
   | LLNil -> ()
   | LLCons x next -> 
     let h0 = get_heap() in 
     assert (h0 `contains` next);
-    sst_share #(SRef (SLList SNat)) next;
+    assert (is_private next h0);
+    admit();
+    sst_share #(SLList SNat) next;
+    assert (is_shared next h0);
     (* let h = get_heap() in *)
     let tl = read next in
     share_llist tl
@@ -143,9 +183,9 @@ let rec auto_grader
   | (gr, hw)::tl -> begin
     let ll = generate_llist l in
     share_llist ll;
-    admit ();
+    (* admit (); *)
     (match hw ll with
-    | Some _ -> sst_write'' gr MaxGrade
-    | None -> sst_write'' gr MinGrade);
+    | Some _ -> sst_write gr MaxGrade
+    | None -> sst_write gr MinGrade);
     auto_grader l tl
   end
